Test/tutorial/ImpVerifiedCompiler/comparison/SequencesTest.dfy
@@ -1,223 +1,224 @@
 abstract module SEQUENCES {
 
 	type T(!new)
+	predicate R(x: T,y: T)
 	
-	least predicate star(R: (T,T) -> bool, conf1: T, conf2: T) {
-		(conf1 == conf2) || (exists conf_inter: T :: R(conf1, conf_inter) && star(R,conf_inter, conf2))
+	least predicate star(conf1: T, conf2: T) {
+		(conf1 == conf2) || (exists conf_inter: T :: R(conf1, conf_inter) && star(conf_inter, conf2))
 	}
 
-	predicate Star(R: (T,T) -> bool, conf1: T, conf2: T) {
-		star(R, conf1, conf2)
+	predicate Star(conf1: T, conf2: T) {
+		star(conf1, conf2)
 	}
 
-	lemma star_one_sequent(R: (T,T) -> bool, conf1: T, conf2: T)
+	lemma star_one_sequent(conf1: T, conf2: T)
 		requires R(conf1,conf2)
-		ensures star(R,conf1,conf2)
+		ensures star(conf1,conf2)
 	{
 	}
 
 	lemma star_one()
-		ensures forall R: (T,T) -> bool :: forall conf1, conf2: T :: R(conf1,conf2) ==> star(R,conf1,conf2)
+		ensures forall R: (T,T) -> bool :: forall conf1, conf2: T :: R(conf1,conf2) ==> star(conf1,conf2)
 	{
 	}
 
-	least lemma star_trans_pre(R: (T,T) -> bool, conf1: T, conf2: T, conf3: T)
-		requires star(R,conf1,conf2)
-		ensures  star(R,conf2,conf3) ==> star(R,conf1,conf3)
+	least lemma star_trans_pre(conf1: T, conf2: T, conf3: T)
+		requires star(conf1,conf2)
+		ensures  star(conf2,conf3) ==> star(conf1,conf3)
 	{
 		if conf1 == conf2 {}
 		else {
-			var confi :| R(conf1, confi) && star(R,confi, conf2);
-			assert star(R,confi,conf2);
-			star_trans_pre(R,confi,conf2,conf3); 
+			var confi :| R(conf1, confi) && star(confi, conf2);
+			assert star(confi,conf2);
+			star_trans_pre(confi,conf2,conf3); 
 		}
 	}
 
-	lemma star_trans_sequent(R: (T,T) -> bool, conf1: T, conf2: T, conf3: T)
-		requires star(R,conf1,conf2) 
-		requires star(R,conf2,conf3)
-		ensures star(R,conf1,conf3)
+	lemma star_trans_sequent(conf1: T, conf2: T, conf3: T)
+		requires star(conf1,conf2) 
+		requires star(conf2,conf3)
+		ensures star(conf1,conf3)
 	{
-		star_trans_pre(R,conf1,conf2,conf3);
+		star_trans_pre(conf1,conf2,conf3);
 	}
 
 	lemma star_trans()
-		ensures forall R: (T,T) -> bool :: forall conf1, conf2, conf3: T :: (star(R,conf1,conf2) && star(R,conf2,conf3)) ==> star(R,conf1,conf3)
+		ensures forall R: (T,T) -> bool :: forall conf1, conf2, conf3: T :: (star(conf1,conf2) && star(conf2,conf3)) ==> star(conf1,conf3)
 	{
-		forall R, conf1, conf2, conf3: T ensures (star(R,conf1,conf2) && star(R,conf2,conf3)) ==> star(R,conf1,conf3) {
-			if star(R,conf1,conf2) {
-				star_trans_pre(R,conf1,conf2,conf3);
+		forall conf1, conf2, conf3: T ensures (star(conf1,conf2) && star(conf2,conf3)) ==> star(conf1,conf3) {
+			if star(conf1,conf2) {
+				star_trans_pre(conf1,conf2,conf3);
 			}
 		}
 	}
 
 	lemma combine_reductions()
-		ensures forall R: (T,T) -> bool :: forall conf1, conf2: T :: R(conf1,conf2) ==> star(R,conf1,conf2)
-		ensures forall R: (T,T) -> bool :: forall conf1, conf2, conf3: T :: (star(R,conf1,conf2) && star(R,conf2,conf3)) ==> star(R,conf1,conf3)
+		ensures forall R: (T,T) -> bool :: forall conf1, conf2: T :: R(conf1,conf2) ==> star(conf1,conf2)
+		ensures forall R: (T,T) -> bool :: forall conf1, conf2, conf3: T :: (star(conf1,conf2) && star(conf2,conf3)) ==> star(conf1,conf3)
 	{
 		star_one();
 		star_trans();
 	}
 
-	least predicate plus(R: (T,T) -> bool, conf1: T, conf2: T) {
-		(exists conf_inter: T :: R(conf1, conf_inter) && star(R,conf_inter, conf2))
+	least predicate plus(conf1: T, conf2: T) {
+		(exists conf_inter: T :: R(conf1, conf_inter) && star(conf_inter, conf2))
 	}
 
-	least predicate Plus(R: (T,T) -> bool, conf1: T, conf2: T) {
-		plus(R,conf1, conf2)
+	least predicate Plus(conf1: T, conf2: T) {
+		plus(conf1, conf2)
 	}
 
-	lemma plus_one(R: (T,T) -> bool, conf1: T, conf2: T)
+	lemma plus_one(conf1: T, conf2: T)
 		requires R(conf1,conf2)
-		ensures star(R,conf1,conf2)
+		ensures star(conf1,conf2)
 	{
 	}
 
-	lemma plus_star(R: (T,T) -> bool, conf1: T, conf2: T)
-		requires plus(R,conf1,conf2)
-		ensures star(R,conf1,conf2)
+	lemma plus_star(conf1: T, conf2: T)
+		requires plus(conf1,conf2)
+		ensures star(conf1,conf2)
 	{
-		var conf1' :| R(conf1, conf1') && star(R,conf1', conf2);
-		star_one_sequent(R,conf1,conf1');
-		star_trans_sequent(R,conf1,conf1',conf2);
+		var conf1' :| R(conf1, conf1') && star(conf1', conf2);
+		star_one_sequent(conf1,conf1');
+		star_trans_sequent(conf1,conf1',conf2);
 	}
 
-	lemma star_plus_trans(R: (T,T) -> bool, conf1: T, conf2: T, conf3: T)
-		requires star(R,conf1,conf2)
-		requires plus(R,conf2,conf3)
-		ensures plus(R,conf1,conf3)
+	lemma star_plus_trans(conf1: T, conf2: T, conf3: T)
+		requires star(conf1,conf2)
+		requires plus(conf2,conf3)
+		ensures plus(conf1,conf3)
 	{
 		if conf1 == conf2 {
 		} else {
-			var conf1' :| R(conf1, conf1') && star(R,conf1', conf2);
-			var conf2' :| R(conf2, conf2') && star(R,conf2', conf3);
-			star_one_sequent(R,conf2,conf2');
-			star_trans_sequent(R,conf1',conf2,conf2');
-			star_trans_sequent(R,conf1',conf2',conf3);
+			var conf1' :| R(conf1, conf1') && star(conf1', conf2);
+			var conf2' :| R(conf2, conf2') && star(conf2', conf3);
+			star_one_sequent(conf2,conf2');
+			star_trans_sequent(conf1',conf2,conf2');
+			star_trans_sequent(conf1',conf2',conf3);
 		}
 	}
 
 
-	predicate all_seq_inf(R: (T,T) -> bool,conf: T) {
-		forall conf2: T :: star(R,conf,conf2) ==> exists conf3: T :: R(conf2,conf3)
+	predicate all_seq_inf(conf: T) {
+		forall conf2: T :: star(conf,conf2) ==> exists conf3: T :: R(conf2,conf3)
 	}
 
-	greatest predicate inf(R: (T,T) -> bool,conf: T) {
-		exists confi: T :: R(conf,confi) && inf(R,confi)
+	greatest predicate inf(conf: T) {
+		exists confi: T :: R(conf,confi) && inf(confi)
 	}
 
-	greatest predicate Inf(R: (T,T) -> bool,conf: T) {
-		inf(R,conf)
+	greatest predicate Inf(conf: T) {
+		inf(conf)
 	}
 
-	least lemma star_inf_trans(R: (T,T) -> bool, conf1: T, conf2: T)
-		requires star(R,conf1,conf2)
-		requires inf(R,conf2)
-		ensures inf(R,conf1)
+	least lemma star_inf_trans(conf1: T, conf2: T)
+		requires star(conf1,conf2)
+		requires inf(conf2)
+		ensures inf(conf1)
 	{
 		if conf1 == conf2 {}
 		else {
-			var conf1' :| R(conf1, conf1') && star(R,conf1', conf2);
-			star_inf_trans(R,conf1',conf2);
+			var conf1' :| R(conf1, conf1') && star(conf1', conf2);
+			star_inf_trans(conf1',conf2);
 		}
 	}
 	
-	greatest lemma infseq_if_all_seq_inf_pre(R: (T,T) -> bool, conf: T)
-		requires forall conf2: T :: star(R,conf,conf2) ==> exists conf3: T :: R(conf2,conf3)
-		ensures inf(R,conf)
+	greatest lemma infseq_if_all_seq_inf_pre(conf: T)
+		requires forall conf2: T :: star(conf,conf2) ==> exists conf3: T :: R(conf2,conf3)
+		ensures inf(conf)
 	{
-		assert star(R,conf,conf);
+		assert star(conf,conf);
 		var B :| R(conf,B);
 		assert R(conf,B);
-		assert inf(R,B) by { infseq_if_all_seq_inf_pre(R,B); }
+		assert inf(B) by { infseq_if_all_seq_inf_pre(B); }
 	}
 
-	lemma infseq_if_all_seq_inf(R: (T,T) -> bool, conf: T)
-		requires all_seq_inf(R,conf)
-		ensures inf(R,conf)
+	lemma infseq_if_all_seq_inf(conf: T)
+		requires all_seq_inf(conf)
+		ensures inf(conf)
 	{
-		infseq_if_all_seq_inf_pre(R,conf);
+		infseq_if_all_seq_inf_pre(conf);
 	}
 
-	lemma infseq_coinduction_principle_ord(k: ORDINAL, R: (T,T) -> bool, X: T -> bool, a : T)
+	lemma infseq_coinduction_principle_ord(k: ORDINAL, X: T -> bool, a : T)
 		requires (forall a: T :: X(a) ==> exists b: T :: R(a,b) && X(b))
 		requires X(a)
-		ensures inf#[k](R,a)
+		ensures inf#[k](a)
 	{
 		if k.Offset == 0 {} else {
 			var b :| R(a,b) && X(b);
-			infseq_coinduction_principle_ord(k-1,R,X,b);
+			infseq_coinduction_principle_ord(k-1,X,b);
 		}
 	}
 
-	predicate {:opaque} always_step(R: (T,T) -> bool, X: T -> bool) {
+	predicate {:opaque} always_step(X: T -> bool) {
 		forall a: T :: X(a) ==> exists b: T :: R(a,b) && X(b)
 	}
 
-	greatest lemma infseq_coinduction_principle_pre(R: (T,T) -> bool, X: T -> bool, a: T)
-		requires always_step(R,X)
-		ensures  X(a) ==> inf(R,a)
+	greatest lemma infseq_coinduction_principle_pre(X: T -> bool, a: T)
+		requires always_step(X)
+		ensures  X(a) ==> inf(a)
 	{
 		reveal always_step();
-		forall a: T ensures X(a) ==> inf(R,a) {
+		forall a: T ensures X(a) ==> inf(a) {
 			if X(a) {
 				var b :| R(a,b) && X(b);
-				infseq_coinduction_principle_pre(R,X,a);
+				infseq_coinduction_principle_pre(X,a);
 			}
 		}
 	}
 
-	lemma infseq_coinduction_principle(R: (T,T) -> bool, X: T -> bool, a : T)
-		requires always_step(R,X)
+	lemma infseq_coinduction_principle(X: T -> bool, a : T)
+		requires always_step(X)
 		requires X(a)
-		ensures inf(R,a)
+		ensures inf(a)
 	{
 		reveal always_step();
 		if X(a) {
-			infseq_coinduction_principle_pre(R,X,a);
+			infseq_coinduction_principle_pre(X,a);
 		}
 		
 	}
 
-	predicate {:opaque} Y(R: (T,T) -> bool, X: T -> bool, a: T) {
-		exists b: T :: star(R,a,b) && X(b)
+	predicate {:opaque} Y(X: T -> bool, a: T) {
+		exists b: T :: star(a,b) && X(b)
 	}
 
-	predicate {:opaque} always_steps(R: (T,T) -> bool, X: T -> bool) {
-		forall a: T :: X(a) ==> exists b: T :: plus(R,a, b) && X(b)
+	predicate {:opaque} always_steps(X: T -> bool) {
+		forall a: T :: X(a) ==> exists b: T :: plus(a, b) && X(b)
 	}
 
-	lemma infseq_coinduction_principle_2_pre_lift(R: (T,T) -> bool, X: T -> bool)
-		requires always_steps(R,X)
-		ensures always_step(R,(a: T) => Y(R,X,a))
+	lemma infseq_coinduction_principle_2_pre_lift(X: T -> bool)
+		requires always_steps(X)
+		ensures always_step((a: T) => Y(X,a))
 	{
 		reveal always_step();
-		forall a: T ensures ((a: T) => Y(R,X,a))(a) ==> exists b: T :: R(a, b) && ((a: T) => Y(R,X,a))(b) {
-			if ((a: T) => Y(R,X,a))(a) {
+		forall a: T ensures ((a: T) => Y(X,a))(a) ==> exists b: T :: R(a, b) && ((a: T) => Y(X,a))(b) {
+			if ((a: T) => Y(X,a))(a) {
 				reveal always_steps();
-				var b :| plus(R,a, b) && X(b);
-				var c :| R(a,c) && star(R,c,b);
+				var b :| plus(a, b) && X(b);
+				var c :| R(a,c) && star(c,b);
 			}
 		}
 	}
 
-	lemma infseq_coinduction_principle_2(R: (T,T) -> bool, X: T -> bool, a : T)
-		requires H1: always_steps(R,X)
+	lemma infseq_coinduction_principle_2(X: T -> bool, a : T)
+		requires H1: always_steps(X)
 		requires H2: X(a)
-		ensures inf(R,a)
+		ensures inf(a)
 	{
 
-		assert Y(R,X,a) by {
+		assert Y(X,a) by {
 			reveal H2;
 			reveal Y();
 		}
 
-		assert always_step(R,(a: T) => Y(R,X,a)) by {
+		assert always_step((a: T) => Y(X,a)) by {
 			reveal H1;
-			infseq_coinduction_principle_2_pre_lift(R,X);
+			infseq_coinduction_principle_2_pre_lift(X);
 		}
 		
-		infseq_coinduction_principle(R,(a: T) => Y(R,X,a),a);
+		infseq_coinduction_principle((a: T) => Y(X,a),a);
 		
 	}
 
