Test/tutorial/ImpVerifiedCompiler/comparison/IMPTest.dfy
@@ -38,107 +38,112 @@ module X refines SEQUENCES {
 
 	import opened Z
 	
-	type T(!new) = (com,cont,store) 
+	type T(!new) = (com,cont,store)
+
+
+	predicate id_in_aexp(id: ident, a: aexp) {
+		match a
+			case AConst(n) => false
+			case AId(id') => id == id'
+			case APlus(a1, a2) => id_in_aexp(id,a1) || id_in_aexp(id,a2)
+			case AMinus(a1, a2) => id_in_aexp(id,a1) || id_in_aexp(id,a2)
+	}
+	
+	function aeval(s: store, a: aexp): int
+		requires forall id: ident :: id_in_aexp(id,a) ==> id in s
+	{
+		match a
+			case AConst(n) => n
+			case AId(id) => s[id]
+			case APlus(a1, a2) => aeval(s,a1) + aeval(s,a2)
+			case AMinus(a1, a2) => aeval(s,a1) - aeval(s,a2)
+	}
+	
+	predicate id_in_bexp(id: ident, b: bexp) {
+		match b
+			case BTrue => true
+			case BFalse => false
+			case BEq(a1,a2) => id_in_aexp(id,a1) || id_in_aexp(id,a2)
+			case BLe(a1,a2) => id_in_aexp(id,a1) || id_in_aexp(id,a2)
+			case BNot(b) => id_in_bexp(id,b)
+			case BAnd(b1,b2) => id_in_bexp(id,b1) || id_in_bexp(id,b2)
+				
+	}
+	
+	function beval(s: store, b: bexp): bool
+		requires forall id: ident :: id_in_bexp(id,b) ==> id in s
+	{
+		match b
+			case BTrue => true
+			case BFalse => false
+			case BEq(a1, a2) => aeval(s,a1) == aeval(s,a2)
+			case BLe(a1, a2) => aeval(s,a1) <= aeval(s,a2)
+			case BNot(b) => ! beval(s,b)
+			case BAnd(b1,b2) => beval(s,b1) && beval(s,b2)
+	}
+	
+	predicate id_in_com(id: ident, c: com) {
+		match c
+			case CSkip => false
+			case CAsgn(id',a) => id_in_aexp(id,a) 
+			case CSeq(c1, c2) => id_in_com(id,c1) || id_in_com(id,c2)
+			case CIf(b,c1,c2) => id_in_bexp(id,b) || id_in_com(id,c1) || id_in_com(id,c2)
+			case CWhile(b,c) => id_in_bexp(id,b) || id_in_com(id,c)
+	}
+
+
+
+	predicate step(conf1: T, conf2: T) {
+		var (c1,k1,s1) := conf1;
+		var (c2,k2,s2) := conf2;
+		match (c1,k1) {
+			case (CAsgn(i, a), _) =>
+				&& (forall id: ident :: id_in_aexp(id,a) ==> id in s1)
+				&& c2 == CSkip
+				&& k2 == k1
+				&& s2 == s1[i := aeval(s1,a)]
+			case (CSeq(c1', c1''), k) =>
+				&& c2 == c1'
+				&& k2 == Kseq(c1'',k)
+				&& s2 == s1
+			case (CIf(b, cifso, cifnotso), _) =>
+				&& (forall id: ident :: id_in_bexp(id,b) ==> id in s1)
+				&& c2 == (if beval(s1, b) then cifso else cifnotso)
+				&& k2 == k1
+				&& s2 == s1
+			case (CWhile(b, c), k) =>
+				&& (forall id: ident :: id_in_bexp(id,b) ==> id in s1)
+				&& c2 == (if beval(s1,b) then c else CSkip)
+				&& k2 == (if beval(s1,b) then Kwhile(b,c,k) else k1)
+				&& s2 == s1
+			case (CSkip, Kseq(c, k)) =>
+				&& c2 == c
+				&& k2 == k
+				&& s2 == s1
+			case (CSkip, Kwhile(b, c, k)) =>
+				&& c2 == CWhile(b,c)
+				&& k2 == k
+				&& s2 == s1
+			case _ => false
+		}
+	}
+		
+	predicate R(x: T, y: T) {
+		step(x,y)
+	}
 
 }
 
 import opened Z
 	
 type conf = X.T
-	
-predicate id_in_aexp(id: ident, a: aexp) {
-	match a
-		case AConst(n) => false
-		case AId(id') => id == id'
-		case APlus(a1, a2) => id_in_aexp(id,a1) || id_in_aexp(id,a2)
-		case AMinus(a1, a2) => id_in_aexp(id,a1) || id_in_aexp(id,a2)
-}
-	
-function aeval(s: store, a: aexp): int
-	requires forall id: ident :: id_in_aexp(id,a) ==> id in s
-{
-	match a
-		case AConst(n) => n
-		case AId(id) => s[id]
-		case APlus(a1, a2) => aeval(s,a1) + aeval(s,a2)
-		case AMinus(a1, a2) => aeval(s,a1) - aeval(s,a2)
-}
-	
-predicate id_in_bexp(id: ident, b: bexp) {
-	match b
-		case BTrue => true
-		case BFalse => false
-		case BEq(a1,a2) => id_in_aexp(id,a1) || id_in_aexp(id,a2)
-		case BLe(a1,a2) => id_in_aexp(id,a1) || id_in_aexp(id,a2)
-		case BNot(b) => id_in_bexp(id,b)
-		case BAnd(b1,b2) => id_in_bexp(id,b1) || id_in_bexp(id,b2)
-			
-}
-	
-function beval(s: store, b: bexp): bool
-	requires forall id: ident :: id_in_bexp(id,b) ==> id in s
-{
-	match b
-		case BTrue => true
-		case BFalse => false
-		case BEq(a1, a2) => aeval(s,a1) == aeval(s,a2)
-		case BLe(a1, a2) => aeval(s,a1) <= aeval(s,a2)
-		case BNot(b) => ! beval(s,b)
-		case BAnd(b1,b2) => beval(s,b1) && beval(s,b2)
-}
-	
-predicate id_in_com(id: ident, c: com) {
-	match c
-		case CSkip => false
-		case CAsgn(id',a) => id_in_aexp(id,a) 
-		case CSeq(c1, c2) => id_in_com(id,c1) || id_in_com(id,c2)
-		case CIf(b,c1,c2) => id_in_bexp(id,b) || id_in_com(id,c1) || id_in_com(id,c2)
-		case CWhile(b,c) => id_in_bexp(id,b) || id_in_com(id,c)
-}
 
-
-
-predicate step(conf1: conf, conf2: conf) {
-	var (c1,k1,s1) := conf1;
-	var (c2,k2,s2) := conf2;
-	match (c1,k1) {
-		case (CAsgn(i, a), _) =>
-			&& (forall id: ident :: id_in_aexp(id,a) ==> id in s1)
-			&& c2 == CSkip
-			&& k2 == k1
-			&& s2 == s1[i := aeval(s1,a)]
-		case (CSeq(c1', c1''), k) =>
-			&& c2 == c1'
-			&& k2 == Kseq(c1'',k)
-			&& s2 == s1
-		case (CIf(b, cifso, cifnotso), _) =>
-			&& (forall id: ident :: id_in_bexp(id,b) ==> id in s1)
-			&& c2 == (if beval(s1, b) then cifso else cifnotso)
-			&& k2 == k1
-			&& s2 == s1
-		case (CWhile(b, c), k) =>
-			&& (forall id: ident :: id_in_bexp(id,b) ==> id in s1)
-			&& c2 == (if beval(s1,b) then c else CSkip)
-			&& k2 == (if beval(s1,b) then Kwhile(b,c,k) else k1)
-			&& s2 == s1
-		case (CSkip, Kseq(c, k)) =>
-			&& c2 == c
-			&& k2 == k
-			&& s2 == s1
-		case (CSkip, Kwhile(b, c, k)) =>
-			&& c2 == CWhile(b,c)
-			&& k2 == k
-			&& s2 == s1
-		case _ => false
-	}
-}
-
-predicate fin_reds(conf1: conf, conf2: conf) {
-	X.star((c1,c2) => step(c1,c2),conf1,conf2)
-}
+// predicate fin_reds(conf1: conf, conf2: conf) {
+// 	X.star(X.R,conf1,conf2)
+// }
 	
-predicate inf_reds(conf: conf) {
-	X.inf((c1,c2) => step(c1,c2),conf)
-}
+// predicate inf_reds(conf: conf) {
+// 	X.inf(X.R,conf)
+// }
 
 
